coq/handwritten/S2N/Embedding.v
@@ -68,6 +68,22 @@ Global Instance Embedding_seq_tuple A B (n : nat) `{Embedding A B}
     toConcrete b := genOrdinal _ _ (fun i => toConcrete (tnth b i));
   |}.
 
+Fixpoint bitvector_to_BITS {n : nat} (s : bitvector n) : BITS n :=
+  match s in Vector.t _ n' return n'.-tuple _ with
+  | nil => [tuple]
+  | cons h _ t => rcons_tuple (bitvector_to_BITS t) h
+  end.
+
+(* NOTE this is risky, Embedding_seq_tuple and Embedding_bitvector_BITS are
+overlapping and not compatible.
+ *)
+Global Instance Embedding_bitvector_BITS (n : nat)
+  : Embedding (bitvector n) (BITS n) :=
+  {|
+    toAbstract c := map_tuple toAbstract (bitvector_to_BITS c);
+    toConcrete b := genOrdinal _ _ (fun i => toConcrete (tnth b (rev_ord i)));
+  |}.
+
 Theorem tnth_rshift {A n} (h : A) (t : n.-tuple A) (i : 'I_n)
   : tnth (cat_tuple [tuple h] t) (rshift 1 i) = tnth t i.
 Proof.
@@ -115,6 +131,179 @@ Proof.
       setoid_rewrite roundtrip.
       setoid_rewrite tnth_rshift.
       apply genOrdinal_tnth.
+    }
+  }
+Qed.
+
+Theorem map_tuple_id {A n} (t : n.-tuple A) : map_tuple Datatypes.id t = t.
+Proof.
+  apply val_inj.
+  move : n t.
+  elim => [|n IH].
+  {
+    move => t.
+    rewrite [t] tuple0.
+    reflexivity.
+  }
+  {
+    case / tupleP => h t.
+    simpl.
+    f_equal.
+    apply IH.
+  }
+Qed.
+
+Theorem tnth_cons_tuple_ord0 {T n} h (t : n.-tuple T)
+  : tnth [tuple of h :: t] ord0 = h.
+Proof.
+  reflexivity.
+Qed.
+
+Theorem decompose_rcons_tuple {T n} h (t : n.-tuple T) l
+  : rcons_tuple [tuple of h :: t] l = [tuple of h :: rcons_tuple t l].
+Proof.
+  apply val_inj => /=.
+  reflexivity.
+Qed.
+
+Theorem nth_rcons_tuple_last {T n} def (tuple : n.-tuple T) last
+  : nth def (rcons_tuple tuple last) n = last.
+Proof.
+  rewrite nth_rcons.
+  rewrite size_tuple.
+  rewrite ltnn.
+  rewrite eqxx.
+  reflexivity.
+Qed.
+
+Theorem tnth_rcons_tuple_rev_ord0 {T n} (tuple : n.-tuple T) last
+  : tnth (rcons_tuple tuple last) (rev_ord ord0) = last.
+Proof.
+  rewrite / tnth /=.
+  rewrite subSS.
+  rewrite subn0.
+  rewrite nth_rcons_tuple_last.
+  reflexivity.
+Qed.
+
+Lemma nth_cons
+      (T : Type) (n : nat) (last : T) (i : nat) (def1 def2 hd : T) (tl : n.-tuple T)
+  : i < size tl ->
+    nth def1 (hd :: tl) i.+1 = nth def2 tl i.
+Proof.
+  move => I /=.
+  by apply set_nth_default.
+Qed.
+
+Theorem ltsubn n i
+  : 0 < i <= n -> n - i < n.
+Proof.
+  move => /andP [? ?].
+  rewrite <- subn_gt0.
+  rewrite subKn //.
+Qed.
+
+(* This comes up a lot... *)
+Theorem ord_lt_le n (i : 'I_n)
+  : 0 < i ->
+    0 < i <= n.
+Proof.
+  move : i => [i I] /= A.
+  rewrite A /=.
+  by apply ltnW.
+Qed.
+
+Lemma nth_rcons_tuple_nat
+      (T : Type) (n : nat) (tuple : n.-tuple T) (last : T) (i : nat) def1 def2
+  : 0 < i <= n ->
+    nth def1 (rcons_tuple tuple last) (n - i)
+    =
+    nth def2 tuple (n - i).
+Proof.
+  move => I.
+  rewrite nth_rcons.
+  rewrite size_tuple.
+  rewrite ltsubn //.
+  apply set_nth_default.
+  rewrite size_tuple.
+  rewrite ltsubn //.
+Qed.
+
+Lemma nth_rcons_tuple_ord
+      (T : Type) (n : nat) (tuple : n.-tuple T) (last : T) (i : 'I_n) def1 def2
+  : 0 < i ->
+    nth def1 (rcons_tuple tuple last) (n - i)
+    =
+    nth def2 tuple (n - i).
+Proof.
+  move => I.
+  erewrite nth_rcons_tuple_nat.
+  {
+    reflexivity.
+  }
+  {
+    by apply ord_lt_le.
+  }
+Qed.
+
+Lemma nth_rev_tuple
+      (T : Type) (n : nat) (tuple : n.-tuple T) (i : 'I_n) def1 def2
+  : nth def1 (rev_tuple tuple) i
+    =
+    nth def2 tuple (n - i.+1).
+Proof.
+  rewrite nth_rev size_tuple //.
+  apply set_nth_default.
+  rewrite size_tuple.
+  apply rev_ord_proof.
+Qed.
+
+Theorem tnth_rcons_tuple_rev_ord_rshift {T n} (tuple : n.-tuple T) last i
+  : tnth (rcons_tuple tuple last) (rev_ord (rshift 1 i)) = tnth (rev_tuple tuple) i.
+Proof.
+  rewrite / tnth.
+  rewrite (lock rcons_tuple) (lock rev_tuple) /=.
+  unlock.
+  rewrite subSS.
+  erewrite nth_rcons_tuple_nat with (def2 := last) => //=.
+  setoid_rewrite nth_rev_tuple => //=.
+Qed.
+
+Theorem rev_tuple_bitvector_to_BITS {n} (v : bitvector n)
+  : rev_tuple (bitvector_to_BITS v) = seq_to_tuple v.
+Proof.
+  apply val_inj.
+  rewrite / rev_tuple / rcons_tuple /=.
+  move : n v.
+  apply Vector.t_ind => [|h n' t IH] //=.
+  rewrite rev_rcons IH //=.
+Qed.
+
+Global Instance ProperEmbedding_bitvector_BITS n
+  : ProperEmbedding (Embedding_bitvector_BITS n).
+Proof.
+  apply Build_ProperEmbedding.
+  move : n.
+  apply Vector.t_ind.
+  {
+    reflexivity.
+  }
+  {
+    move => h n t IH.
+    simpl.
+    f_equal.
+    {
+      rewrite map_tuple_id.
+      rewrite tnth_rcons_tuple_rev_ord0.
+      reflexivity.
+    }
+    {
+      setoid_rewrite tnth_map.
+      erewrite genOrdinal_domain_eq; [ apply genOrdinal_tnth | ].
+      move => i /=.
+      rewrite tnth_rcons_tuple_rev_ord_rshift.
+      f_equal.
+      apply rev_tuple_bitvector_to_BITS.
     }
   }
 Qed.
