coq/handwritten/SAWCoreScaffolding.v
@@ -1,6 +1,9 @@
-From Coq.Lists          Require Import List.
-From Coq.Numbers.NatInt Require        NZLog.
-From Coq.Strings        Require        String.
+From Coq Require Import Numbers.Cyclic.ZModulo.ZModulo.
+From Coq Require Import ZArith.BinInt.
+From Coq Require Import ZArith.Zdiv.
+From Coq Require Import Lists.List.
+From Coq Require        Numbers.NatInt.NZLog.
+From Coq Require        Strings.String.
 
 Definition sort (n : nat) := Type.
 
@@ -162,15 +165,13 @@ Definition snd {A B} := @snd A B.
 Definition Zero := O.
 Definition Succ := S.
 
-From Coq Require Import ZArith.BinInt.
-From Coq Require Import ZArith.Zdiv.
 
 Definition Integer := Z.
-Definition intAdd : Integer -> Integer -> Integer := Zplus.
-Definition intSub : Integer -> Integer -> Integer := Zminus.
-Definition intMul : Integer -> Integer -> Integer := Zmult.
+Definition intAdd : Integer -> Integer -> Integer := Z.add.
+Definition intSub : Integer -> Integer -> Integer := Z.sub.
+Definition intMul : Integer -> Integer -> Integer := Z.mul.
 Definition intDiv : Integer -> Integer -> Integer := Z.div.
-Definition intMod : Integer -> Integer -> Integer := Zmod.
+Definition intMod : Integer -> Integer -> Integer := Z.modulo.
 Definition intMin : Integer -> Integer -> Integer := Z.min.
 Definition intMax : Integer -> Integer -> Integer := Z.max.
 Definition intNeg : Integer -> Integer := Z.opp.
@@ -181,11 +182,9 @@ Definition intLt : Integer -> Integer -> Bool := Z.ltb.
 Definition intToNat : Integer -> Nat := Z.to_nat.
 Definition natToInt : Nat -> Integer := Z.of_nat.
 
-From Coq Require Import Numbers.Cyclic.ZModulo.ZModulo.
-
 (* NOTE: the following will be nonsense for values of n <= 1 *)
 Definition IntMod (n : nat) := Z.
-Definition toIntMod (n : Nat) : Integer -> IntMod n := fun i => Zmod i (Z.of_nat n).
+Definition toIntMod (n : Nat) : Integer -> IntMod n := fun i => Z.modulo i (Z.of_nat n).
 Definition fromIntMod (n : Nat) : (IntMod n) -> Integer := ZModulo.to_Z (Pos.of_nat n).
 Local Notation "[| a |]_ n" := (to_Z (Pos.of_nat n) a) (at level 0, a at level 99).
 Definition intModEq (n : Nat) (a : IntMod n) (b : IntMod n) : Bool
